theories/c_toy_lang/notation.v
@@ -58,7 +58,7 @@ Notation "'while:' e1 'do' e2" := (While e1%E e2%E)
   (at level 200, e1, e2 at level 200) : expr_scope.
 
 Notation "'call:' ff 'with' '(' e1 , .. , en ')'" := (FunCall ff%E (cons e1%E .. (cons en%E nil) ..))
-  (at level 200, ff, e1, en at level 200) : expr_scope.
+  (at level 200, ff, e1, en at level 99) : expr_scope.
 
 Notation "'let:' x := e1 'in' e2" := (Let x%binder e1%E e2%E)
   (at level 200, x at level 1, e1, e2 at level 200,
